chore: build correct safety, liveness circuits. We still need to show that what we build matches the FSM specs

SSA/Experimental/Bits/Fast/Circuit.lean
@@ -442,43 +442,35 @@ def bAnd : ∀ (_s : List α) (_f : α → Circuit β), Circuit β
     rw [bAnd, eval_foldl_and]; simp
 
 /-- perform the same task as assignVars, but don't change the signature of the circuit. -/
-def assignVars' [DecidableEq α] (c : Circuit α)
-  (f : ∀ (a : α), Option Bool) : Circuit α
+def assignAllVars [DecidableEq α] (c : Circuit α)
+  (f : α → Bool) : Circuit Empty
   := match c with
   | tru => tru
   | fals => fals
   | var b x =>
-    match f x with
-    | .some v => Circuit.ofBool (b = v)
-    | .none => var b x
-  | and p q => assignVars' p f &&& assignVars' q f
-  | or p q => assignVars' p f ||| assignVars' q f
-  | xor p q => assignVars' p f ^^^ assignVars' q f
+    let v := f x
+    Circuit.ofBool (b = v)
+  | and p q => assignAllVars p f &&& assignAllVars q f
+  | or p q => assignAllVars p f ||| assignAllVars q f
+  | xor p q => assignAllVars p f ^^^ assignAllVars q f
 
 /-- Says how to evaluate asssignVars' in terms of an updated environment. -/
-lemma eval_assignVars'_of_eq [DecidableEq α] {c : Circuit α}
-    {f : (a : α) → Option Bool} {env : α → Bool} {env' : α → Bool}
-    (henv' : env' = (fun x =>
-      match f x with
-      | some v => v
-      | none => env x)) :
-    eval (assignVars' c f) env = c.eval env' := by
-  subst henv'
+@[simp]
+lemma eval_assignAllVars [DecidableEq α] {c : Circuit α} {f : α → Bool} :
+    eval (assignAllVars c f) env = c.eval f := by
   induction c
-  case tru => simp [eval, assignVars']
-  case fals => simp [eval, assignVars']
+  case tru => simp [eval, assignAllVars]
+  case fals => simp [eval, assignAllVars]
   case var b x =>
-    simp [assignVars']
-    rcases fx : f x
-    case none => simp
-    case some v =>
-      rcases v <;> rcases b <;> simp
+    simp [assignAllVars]
+    rcases fx : f x <;> rcases b <;> simp
   case and p q hp hq =>
-    simp [eval, hp, hq, assignVars']
+    simp [eval, hp, hq, assignAllVars]
   case or p q hp hq =>
-    simp [eval, hp, hq, assignVars']
+    simp [eval, hp, hq, assignAllVars]
   case xor p q hp hq =>
-    simp [eval, hp, hq, assignVars']
+    simp [eval, hp, hq, assignAllVars]
+
 
 def assignVars [DecidableEq α] :
     ∀ (c : Circuit α) (_f : ∀ (a : α) (_ha : a ∈ c.vars), β ⊕ Bool), Circuit β
